proof/agp32CorrectScript.sml
@@ -1,4 +1,4 @@
-open hardwarePreamble agp32StateTheory agp32EnvironmentTheory agp32ProcessorTheory ag32Theory ag32ExtraTheory agp32RelationTheory;
+open hardwarePreamble translatorTheory translatorLib arithmeticTheory dep_rewrite blastLib bitstringSyntax fcpSyntax listSyntax wordsSyntax agp32StateTheory agp32EnvironmentTheory agp32ProcessorTheory ag32Theory ag32ExtraTheory agp32RelationTheory;
 
 val _ = new_theory "agp32Correct";
 
@@ -9,6 +9,71 @@ val _ = new_theory "agp32Correct";
 
 val _ = prefer_num ();
 val _ = guess_lengths ();
+
+fun v2w_word_bit_list_cleanup tm =
+  if is_var tm orelse is_const tm then
+    raise UNCHANGED
+  else if is_v2w tm andalso (is_list (rand tm)) then let
+    val (arg, worddim) = dest_v2w tm
+    val (arg, _) = dest_list arg
+    val len = length arg
+  in
+    if len = 1 then
+      raise UNCHANGED
+    else let
+      (* TODO: Fails on lists of non-dest_word_bit calls *)
+      val (hindex, var) = arg |> hd |> dest_word_bit
+      val (lindex, _) = arg |> last |> dest_word_bit
+    in
+      mk_eq (tm, mk_word_extract (hindex, lindex, var, mk_int_numeric_type len)) |> BBLAST_PROVE
+    end
+  end else if is_comb tm then
+    COMB_CONV v2w_word_bit_list_cleanup tm
+  else (* must be abs *)
+    ABS_CONV v2w_word_bit_list_cleanup tm;
+
+(* lemmas about the Silver ISA *)
+Theorem ALU_state_eq_after:
+  !func input1 input2 res a a'.
+    ALU (func, input1, input2) a = (res, a') ==>
+    a'.PC = a.PC /\ a'.MEM = a.MEM /\ a'.PC = a.PC /\ a'.R = a.R /\
+    a'.data_in = a.data_in /\ a'.data_out = a.data_out /\ a'.io_events = a.io_events
+Proof
+  rw [ALU_def] >> Cases_on `func'` >> fs [] >> rw []
+QED
+
+Theorem ag32_data_in_unchanged:
+  !a n. (FUNPOW Next n a).data_in = (FUNPOW Next (SUC n) a).data_in
+Proof
+  rw [FUNPOW_SUC] >>
+  Q.ABBREV_TAC `a1 = FUNPOW Next n a` >>
+  rw [Next_def] >>
+  Q.ABBREV_TAC `i = (a1.MEM ((31 >< 2) a1.PC @@ (0w:word2) + 3w) @@
+                     a1.MEM ((31 >< 2) a1.PC @@ (0w:word2) + 2w) @@
+                     a1.MEM ((31 >< 2) a1.PC @@ (0w:word2) + 1w) @@
+                     a1.MEM ((31 >< 2) a1.PC @@ (0w:word2)))` >>
+  rw [Decode_def,boolify32_def] >> CONV_TAC v2w_word_bit_list_cleanup >>
+  rw [Run_def,dfn'LoadUpperConstant_def,dfn'LoadConstant_def,
+      dfn'Interrupt_def,incPC_def] >-
+   (** JumpIfZero **)
+   (rw [dfn'JumpIfZero_def] >>
+    qpat_abbrev_tac `alu = ALU _ _` >>
+    Cases_on `alu` >> rw [incPC_def] >>
+    METIS_TAC [ALU_state_eq_after]) >-
+   (** JumpIfNotZero **)
+    (rw [dfn'JumpIfNotZero_def] >>
+     qpat_abbrev_tac `alu = ALU _ _` >>
+     Cases_on `alu` >> rw [incPC_def] >>
+     METIS_TAC [ALU_state_eq_after]) >>
+  Cases_on `DecodeReg_imm (v2w [word_bit 31 i],(30 >< 25) i)` >> rw [] >>
+  (** Other instructions **)
+  rw [dfn'Normal_def,norm_def,dfn'Shift_def,incPC_def,dfn'StoreMEM_def,
+      dfn'StoreMEMByte_def,dfn'LoadMEM_def,dfn'LoadMEMByte_def,
+      dfn'Out_def,dfn'In_def,dfn'Accelerator_def,dfn'Jump_def] >>
+  qpat_abbrev_tac `alu = ALU _ _` >>
+  Cases_on `alu` >> rw [] >>
+  METIS_TAC [ALU_state_eq_after]
+QED
 
 Theorem agp32_Init_implies_Rel:
   !k fext fbits s a I.
@@ -37,7 +102,7 @@ Proof
 QED
 
 Theorem agp32_Rel_ag32_correct:
-  !(k:num) fext fbits s a (t:num) i I C.
+  !k fext fbits s a (t:num) I C.
     k >= 1 ==>
     k <= 5 ==>
     s = agp32 fext fbits ==>
@@ -45,23 +110,28 @@ Theorem agp32_Rel_ag32_correct:
     is_mem fext_accessor_circuit s fext ==>
     is_acc accelerator_f s ==>
     is_interrupt_interface fext_accessor_circuit s fext ==>
+    is_data_in fext ==>
     (* cache oracle can introduce hit/miss *)
     (!t. C (s t).data_addr (s t).data_wstrb (s t).data_wdata (s t).command (s t).PC <=> (fext t).ready) ==>
     Init (fext 0) (s 0) a ==>
     (** properties of scheduling function I **)
-    (!t k. enable_stg k (s t) ==> I(k,t) = I(k,t-1) + 1) ==>
+    (!t k. enable_stg k (s (SUC t)) ==> I(k,SUC t) = I(k,t) + 1) ==>
     I(k,0) = 0 ==>
-    I(k,t) = i ==>
-    Rel (fext t) (s t) k a i
+    Rel (fext t) (s t) k a (I(k,t))
 Proof
   rpt strip_tac >>
-  Induct_on `t` >>
-  rpt strip_tac >-
+  Induct_on `t` >> fs [] >-
    METIS_TAC [agp32_Init_implies_Rel] >>
-  fs [Init_def,Rel_def] >>
-  Cases_on `k = 1` >-
-   (** IF stage **)
-   (fs [] >> rw [] >> cheat) >>
+  Q.ABBREV_TAC `i = I'(k,t)` >>
+  Cases_on `enable_stg k (s (SUC t))` >-
+   (`I'(k, SUC t) = SUC i` by fs [] >> fs [Rel_def] >>
+    Cases_on `k = 1` >-
+     (** IF stage **)
+     (fs [] >> rw [] >|[
+         fs [GSYM ag32_data_in_unchanged,is_data_in_def],
+         rw [agp32_def,mk_module_def] >> cheat,
+         cheat]) >>
+      cheat) >>
   cheat
 QED
 
